Added big step evaluation, some derived combinators

BananasLanguage.thy
@@ -16,8 +16,8 @@ and funct =
 
 datatype expr = 
   \<epsilon> | Comp expr expr (infixr "\<cdot>" 65)
-| \<pi>\<^sub>1 | \<pi>\<^sub>2 | \<Delta> | Pairwise expr expr (infix "\<parallel>" 80)
-| \<iota>\<^sub>l | \<iota>\<^sub>r | Case expr expr (infix "\<nabla>" 80)
+| \<pi>\<^sub>1 | \<pi>\<^sub>2 | \<Theta> | Pairwise expr expr (infix "\<parallel>" 80)
+| \<iota>\<^sub>l | \<iota>\<^sub>r | \<Xi> |  Case expr expr (infix "\<bar>" 80)
 | Apply | Arrow expr expr (infix "\<leftarrow>" 70)
 | Outj funct
 
@@ -41,11 +41,12 @@ inductive typecheck\<^sub>e :: "expr \<Rightarrow> type \<Rightarrow> type \<Rig
 | tc_comp [simp]: "f \<turnstile> t\<^sub>2 \<rightarrow> t\<^sub>3 \<Longrightarrow> g \<turnstile> t\<^sub>1 \<rightarrow> t\<^sub>2 \<Longrightarrow> f \<cdot> g \<turnstile> t\<^sub>1 \<rightarrow> t\<^sub>3"
 | tc_fst [simp]: "\<pi>\<^sub>1 \<turnstile> t\<^sub>1 \<otimes> t\<^sub>2 \<rightarrow> t\<^sub>1"
 | tc_snd [simp]: "\<pi>\<^sub>2 \<turnstile> t\<^sub>1 \<otimes> t\<^sub>2 \<rightarrow> t\<^sub>2"
-| tc_tup [simp]: "\<Delta> \<turnstile> t \<rightarrow> t \<otimes> t"
+| tc_tup [simp]: "\<Theta> \<turnstile> t \<rightarrow> t \<otimes> t"
 | tc_pair [simp]: "f\<^sub>1 \<turnstile> t\<^sub>1 \<rightarrow> t\<^sub>2 \<Longrightarrow> f\<^sub>2 \<turnstile> t\<^sub>3 \<rightarrow> t\<^sub>4 \<Longrightarrow> f\<^sub>1 \<parallel> f\<^sub>2 \<turnstile> t\<^sub>1 \<otimes> t\<^sub>3 \<rightarrow> t\<^sub>2 \<otimes> t\<^sub>4"
 | tc_inl [simp]: "\<iota>\<^sub>l \<turnstile> t\<^sub>1 \<rightarrow> t\<^sub>1 \<oplus> t\<^sub>2"
 | tc_inr [simp]: "\<iota>\<^sub>r \<turnstile> t\<^sub>2 \<rightarrow> t\<^sub>1 \<oplus> t\<^sub>2"
-| tc_case [simp]: "f\<^sub>l \<turnstile> t\<^sub>1 \<rightarrow> t\<^sub>3 \<Longrightarrow> f\<^sub>r \<turnstile> t\<^sub>2 \<rightarrow> t\<^sub>3 \<Longrightarrow> f\<^sub>l \<nabla> f\<^sub>r \<turnstile> t\<^sub>1 \<oplus> t\<^sub>2 \<rightarrow> t\<^sub>3"
+| tc_str [simp]: "\<Xi> \<turnstile> t\<^sub>1 \<oplus> t\<^sub>1 \<rightarrow> t\<^sub>1"
+| tc_case [simp]: "f\<^sub>l \<turnstile> t\<^sub>1 \<rightarrow> t\<^sub>3 \<Longrightarrow> f\<^sub>r \<turnstile> t\<^sub>2 \<rightarrow> t\<^sub>4 \<Longrightarrow> f\<^sub>l \<bar> f\<^sub>r \<turnstile> t\<^sub>1 \<oplus> t\<^sub>2 \<rightarrow> t\<^sub>3 \<oplus> t\<^sub>4"
 | tc_app [simp]: "Apply \<turnstile> (t\<^sub>1 \<hookrightarrow> t\<^sub>2) \<otimes> t\<^sub>1 \<rightarrow> t\<^sub>2"
 | tc_arr [simp]: "f \<turnstile> t\<^sub>1 \<rightarrow> t\<^sub>2 \<Longrightarrow> g \<turnstile> t\<^sub>3 \<rightarrow> t\<^sub>4 \<Longrightarrow> g \<leftarrow> f \<turnstile> t\<^sub>2 \<hookrightarrow> t\<^sub>3 \<rightarrow> t\<^sub>1 \<hookrightarrow> t\<^sub>4"
 | tc_outj [simp]: "Outj f \<turnstile> \<mu> f \<rightarrow> f \<star> \<mu> f"
@@ -54,11 +55,12 @@ inductive_cases [elim]: "\<epsilon> \<turnstile> t \<rightarrow> t'"
 inductive_cases [elim]: "f \<cdot> g \<turnstile> t \<rightarrow> t'"
 inductive_cases [elim]: "\<pi>\<^sub>1 \<turnstile> t \<rightarrow> t'"
 inductive_cases [elim]: "\<pi>\<^sub>2 \<turnstile> t \<rightarrow> t'"
-inductive_cases [elim]: "\<Delta> \<turnstile> t \<rightarrow> t'"
+inductive_cases [elim]: "\<Theta> \<turnstile> t \<rightarrow> t'"
 inductive_cases [elim]: "f\<^sub>l \<parallel> f\<^sub>r \<turnstile> t \<rightarrow> t'"
 inductive_cases [elim]: "\<iota>\<^sub>l \<turnstile> t \<rightarrow> t'"
 inductive_cases [elim]: "\<iota>\<^sub>r \<turnstile> t \<rightarrow> t'"
-inductive_cases [elim]: "f\<^sub>l \<nabla> f\<^sub>r \<turnstile> t \<rightarrow> t'"
+inductive_cases [elim]: "\<Xi> \<turnstile> t \<rightarrow> t'"
+inductive_cases [elim]: "f\<^sub>l \<bar> f\<^sub>r \<turnstile> t \<rightarrow> t'"
 inductive_cases [elim]: "Apply \<turnstile> t \<rightarrow> t'"
 inductive_cases [elim]: "g \<leftarrow> f \<turnstile> t \<rightarrow> t'"
 inductive_cases [elim]: "Outj f \<turnstile> t \<rightarrow> t'"
@@ -88,11 +90,13 @@ inductive evaluate :: "expr \<Rightarrow> val \<Rightarrow> expr \<Rightarrow> v
 | ev_pair1 [simp]: "f\<^sub>1 \<cdot> v\<^sub>1 \<leadsto> f\<^sub>1' \<cdot> v\<^sub>1' \<Longrightarrow> f\<^sub>1 \<parallel> f\<^sub>2 \<cdot> PairV v\<^sub>1 v\<^sub>2 \<leadsto> f\<^sub>1' \<parallel> f\<^sub>2 \<cdot> PairV v\<^sub>1' v\<^sub>2"
 | ev_pair2 [simp]: "f\<^sub>2 \<cdot> v\<^sub>2 \<leadsto> f\<^sub>2' \<cdot> v\<^sub>2' \<Longrightarrow> \<epsilon> \<parallel> f\<^sub>2 \<cdot> PairV v\<^sub>1 v\<^sub>2 \<leadsto> \<epsilon> \<parallel> f\<^sub>2' \<cdot> PairV v\<^sub>1 v\<^sub>2'"
 | ev_pair3 [simp]: "\<epsilon> \<parallel> \<epsilon> \<cdot> PairV v\<^sub>1 v\<^sub>2 \<leadsto> \<epsilon> \<cdot> PairV v\<^sub>1 v\<^sub>2"
-| ev_tup [simp]: "\<Delta> \<cdot> v \<leadsto> \<epsilon> \<cdot> PairV v v"
+| ev_tup [simp]: "\<Theta> \<cdot> v \<leadsto> \<epsilon> \<cdot> PairV v v"
 | ev_inl [simp]: "\<iota>\<^sub>l \<cdot> v \<leadsto> \<epsilon> \<cdot> InlV v"
 | ev_inr [simp]: "\<iota>\<^sub>r \<cdot> v \<leadsto> \<epsilon> \<cdot> InrV v"
-| ev_csl [simp]: "f\<^sub>l \<nabla> f\<^sub>r \<cdot> InlV v \<leadsto> f\<^sub>l \<cdot> v"
-| ev_csr [simp]: "f\<^sub>l \<nabla> f\<^sub>r \<cdot> InrV v \<leadsto> f\<^sub>r \<cdot> v"
+| ev_strl [simp]: "\<Xi> \<cdot> InlV v \<leadsto> \<epsilon> \<cdot> v"
+| ev_strr [simp]: "\<Xi> \<cdot> InrV v \<leadsto> \<epsilon> \<cdot> v"
+| ev_csl [simp]: "f\<^sub>l \<bar> f\<^sub>r \<cdot> InlV v \<leadsto> (\<iota>\<^sub>l \<cdot> f\<^sub>l) \<cdot> v"
+| ev_csr [simp]: "f\<^sub>l \<bar> f\<^sub>r \<cdot> InrV v \<leadsto> (\<iota>\<^sub>r \<cdot> f\<^sub>r) \<cdot> v"
 | ev_app [simp]: "Apply \<cdot> PairV (FunV e) v \<leadsto> e \<cdot> v"
 | ev_arr [simp]: "g \<leftarrow> f \<cdot> FunV e \<leadsto> \<epsilon> \<cdot> FunV (g \<cdot> e \<cdot> f)"
 | ev_out [simp]: "Outj f \<cdot> InjV f v \<leadsto> \<epsilon> \<cdot> v"
@@ -138,7 +142,7 @@ theorem progress: "e \<turnstile> t\<^sub>1 \<rightarrow> t\<^sub>2 \<Longrighta
     hence "\<pi>\<^sub>2 \<cdot> v \<leadsto> \<epsilon> \<cdot> v\<^sub>2" by simp
     thus ?case by fastforce
   next case (tc_tup t)
-    hence "\<Delta> \<cdot> v \<leadsto> \<epsilon> \<cdot> PairV v v" by simp
+    hence "\<Theta> \<cdot> v \<leadsto> \<epsilon> \<cdot> PairV v v" by simp
     thus ?case by fastforce
   next case (tc_pair f\<^sub>1 t\<^sub>1 t\<^sub>2 f\<^sub>2 t\<^sub>3 t\<^sub>4)
     then obtain v\<^sub>1 v\<^sub>2 where V: "v\<^sub>1 \<turnstile> t\<^sub>1 \<and> v\<^sub>2 \<turnstile> t\<^sub>3 \<and> v = PairV v\<^sub>1 v\<^sub>2" using canonical_prod by blast
@@ -166,15 +170,26 @@ theorem progress: "e \<turnstile> t\<^sub>1 \<rightarrow> t\<^sub>2 \<Longrighta
   next case (tc_inr t\<^sub>2 t\<^sub>1)
     hence "\<iota>\<^sub>r \<cdot> v \<leadsto> \<epsilon> \<cdot> InrV v" by simp
     thus ?case by fastforce
+  next case tc_str
+    then obtain v' where V: "v = InlV v' \<or> v = InrV v'" using canonical_sum by blast
+    thus ?case
+      proof (cases "v = InlV v'")
+      case True
+        hence "\<Xi> \<cdot> v \<leadsto> \<epsilon> \<cdot> v'" by simp
+        thus ?thesis by fastforce
+      next case False
+        with V have "\<Xi> \<cdot> v \<leadsto> \<epsilon> \<cdot> v'" by simp
+        thus ?thesis by fastforce
+      qed
   next case (tc_case f\<^sub>l t\<^sub>1 t\<^sub>3 f\<^sub>r t\<^sub>2)
     then obtain v' where V: "v = InlV v' \<or> v = InrV v'" using canonical_sum by blast
     thus ?case
       proof (cases "v = InlV v'")
       case True
-        hence "f\<^sub>l \<nabla> f\<^sub>r \<cdot> v \<leadsto> f\<^sub>l \<cdot> v'" by simp
+        hence "f\<^sub>l \<bar> f\<^sub>r \<cdot> v \<leadsto> (\<iota>\<^sub>l \<cdot> f\<^sub>l) \<cdot> v'" by simp
         thus ?thesis by fastforce
       next case False
-        with V have "f\<^sub>l \<nabla> f\<^sub>r \<cdot> v \<leadsto> f\<^sub>r \<cdot> v'" by simp
+        with V have "f\<^sub>l \<bar> f\<^sub>r \<cdot> v \<leadsto> (\<iota>\<^sub>r \<cdot> f\<^sub>r) \<cdot> v'" by simp
         thus ?thesis by fastforce
       qed
   next case (tc_app t\<^sub>1 t\<^sub>2)
@@ -216,11 +231,84 @@ theorem preservation: "e \<cdot> v \<leadsto> e' \<cdot> v' \<Longrightarrow> e 
     moreover then obtain t\<^sub>3 where "t\<^sub>2 = t\<^sub>3 \<oplus> t\<^sub>1" by fastforce
     ultimately have "(\<epsilon> \<turnstile> t\<^sub>3 \<oplus> t\<^sub>1 \<rightarrow> t\<^sub>2) \<and> InrV v \<turnstile> t\<^sub>3 \<oplus> t\<^sub>1" by simp
     thus ?case by fastforce
+  next case (ev_csl f\<^sub>l f\<^sub>r v)
+    then obtain t\<^sub>1\<^sub>l t\<^sub>1\<^sub>r t\<^sub>2\<^sub>l t\<^sub>2\<^sub>r where V: "(f\<^sub>l \<turnstile> t\<^sub>1\<^sub>l \<rightarrow> t\<^sub>2\<^sub>l) \<and> (f\<^sub>r \<turnstile> t\<^sub>1\<^sub>r \<rightarrow> t\<^sub>2\<^sub>r) \<and> (v \<turnstile> t\<^sub>1\<^sub>l) \<and>
+      t\<^sub>1 = t\<^sub>1\<^sub>l \<oplus> t\<^sub>1\<^sub>r \<and> t\<^sub>2 = t\<^sub>2\<^sub>l \<oplus> t\<^sub>2\<^sub>r" by fastforce
+    hence "\<iota>\<^sub>l \<cdot> f\<^sub>l \<turnstile> t\<^sub>1\<^sub>l \<rightarrow> t\<^sub>2\<^sub>l \<oplus> t\<^sub>2\<^sub>r" by (metis tc_inl tc_comp)
+    with V show ?case by fastforce
+  next case (ev_csr f\<^sub>l f\<^sub>r v)
+    then obtain t\<^sub>1\<^sub>l t\<^sub>1\<^sub>r t\<^sub>2\<^sub>l t\<^sub>2\<^sub>r where V: "(f\<^sub>l \<turnstile> t\<^sub>1\<^sub>l \<rightarrow> t\<^sub>2\<^sub>l) \<and> (f\<^sub>r \<turnstile> t\<^sub>1\<^sub>r \<rightarrow> t\<^sub>2\<^sub>r) \<and> (v \<turnstile> t\<^sub>1\<^sub>r) \<and>
+      t\<^sub>1 = t\<^sub>1\<^sub>l \<oplus> t\<^sub>1\<^sub>r \<and> t\<^sub>2 = t\<^sub>2\<^sub>l \<oplus> t\<^sub>2\<^sub>r" by fastforce
+    hence "\<iota>\<^sub>r \<cdot> f\<^sub>r \<turnstile> t\<^sub>1\<^sub>r \<rightarrow> t\<^sub>2\<^sub>l \<oplus> t\<^sub>2\<^sub>r" by (metis tc_inr tc_comp)
+    with V show ?case by fastforce
   next case (ev_arr g f e)
     then obtain t\<^sub>1\<^sub>1 t\<^sub>1\<^sub>2 t\<^sub>2\<^sub>1 t\<^sub>2\<^sub>2 where "(f \<turnstile> t\<^sub>2\<^sub>1 \<rightarrow> t\<^sub>1\<^sub>1) \<and> (g \<turnstile> t\<^sub>1\<^sub>2 \<rightarrow> t\<^sub>2\<^sub>2) \<and> (e \<turnstile> t\<^sub>1\<^sub>1 \<rightarrow> t\<^sub>1\<^sub>2) \<and>
       t\<^sub>1 = t\<^sub>1\<^sub>1 \<hookrightarrow> t\<^sub>1\<^sub>2 \<and> t\<^sub>2 = t\<^sub>2\<^sub>1 \<hookrightarrow> t\<^sub>2\<^sub>2" by fastforce
     hence "(\<epsilon> \<turnstile> t\<^sub>2\<^sub>1 \<hookrightarrow> t\<^sub>2\<^sub>2 \<rightarrow> t\<^sub>2) \<and> FunV (g \<cdot> e \<cdot> f) \<turnstile> t\<^sub>2\<^sub>1 \<hookrightarrow> t\<^sub>2\<^sub>2" by fastforce
     thus ?case by fastforce
   qed force+
- 
+
+(* big-step evaluation *) 
+
+inductive total_eval :: "expr \<Rightarrow> val \<Rightarrow> val \<Rightarrow> bool" (infix "\<cdot> _ \<Down>" 60) where
+  tev_base [simp]: "\<epsilon> \<cdot> v \<Down> v"
+| tev_step [simp]: "e \<cdot> v \<leadsto> e' \<cdot> v' \<Longrightarrow> e' \<cdot> v' \<Down> v'' \<Longrightarrow> e \<cdot> v \<Down> v''"
+
+lemma [elim]: "f \<cdot> v \<Down> v' \<Longrightarrow> g \<cdot> v' \<Down> v'' \<Longrightarrow> (g \<cdot> f) \<cdot> v \<Down> v''"
+  proof (induction f v v' rule: total_eval.induct)
+  case (tev_base v)
+    moreover have "(g \<cdot> \<epsilon>) \<cdot> v \<leadsto> g \<cdot> v" by simp
+    ultimately show ?case by (metis tev_step)
+  next case (tev_step f v f' v' v''')
+    hence "(g \<cdot> f) \<cdot> v \<leadsto> (g \<cdot> f') \<cdot> v'" by simp
+    moreover from tev_step have "(g \<cdot> f') \<cdot> v' \<Down> v''" by simp
+    ultimately show ?case by (metis total_eval.tev_step)
+  qed
+
+lemma [simp]: "e \<cdot> v \<leadsto> \<epsilon> \<cdot> v' \<Longrightarrow> e \<cdot> v \<Down> v'"
+  by rule (simp, simp)
+
+lemma [elim]: "\<epsilon> \<cdot> v \<Down> v' \<Longrightarrow> v = v'"
+  proof (induction \<epsilon> v v' rule: total_eval.induct)
+  case (tev_step v e' v' v'')
+    thus ?case by (induction \<epsilon> v e' v' rule: evaluate.induct)
+  qed simp_all
+
+lemma [simp]: "f\<^sub>2 \<cdot> v\<^sub>2 \<Down> v\<^sub>4 \<Longrightarrow> \<epsilon> \<parallel> f\<^sub>2 \<cdot> PairV v\<^sub>1 v\<^sub>2 \<Down> PairV v\<^sub>1 v\<^sub>4"
+  proof (induction f\<^sub>2 v\<^sub>2 v\<^sub>4 rule: total_eval.induct)
+  case (tev_step f\<^sub>2 v\<^sub>2 f\<^sub>2' v\<^sub>2' v\<^sub>4)
+    hence "\<epsilon> \<parallel> f\<^sub>2 \<cdot> PairV v\<^sub>1 v\<^sub>2 \<leadsto> \<epsilon> \<parallel> f\<^sub>2' \<cdot> PairV v\<^sub>1 v\<^sub>2'" by simp
+    moreover from tev_step have "\<epsilon> \<parallel> f\<^sub>2' \<cdot> PairV v\<^sub>1 v\<^sub>2' \<Down> PairV v\<^sub>1 v\<^sub>4" by simp
+    ultimately show ?case by simp
+  qed simp_all
+
+lemma [simp]: "f\<^sub>1 \<cdot> v\<^sub>1 \<Down> v\<^sub>3 \<Longrightarrow> f\<^sub>2 \<cdot> v\<^sub>2 \<Down> v\<^sub>4 \<Longrightarrow> f\<^sub>1 \<parallel> f\<^sub>2 \<cdot> PairV v\<^sub>1 v\<^sub>2 \<Down> PairV v\<^sub>3 v\<^sub>4"
+  proof (induction f\<^sub>1 v\<^sub>1 v\<^sub>3 rule: total_eval.induct)
+  case (tev_step f\<^sub>1 v\<^sub>1 f\<^sub>1' v\<^sub>1' v\<^sub>3)
+    hence "f\<^sub>1 \<parallel> f\<^sub>2 \<cdot> PairV v\<^sub>1 v\<^sub>2 \<leadsto> f\<^sub>1' \<parallel> f\<^sub>2 \<cdot> PairV v\<^sub>1' v\<^sub>2" by simp
+    moreover from tev_step have "f\<^sub>1' \<parallel> f\<^sub>2 \<cdot> PairV v\<^sub>1' v\<^sub>2 \<Down> PairV v\<^sub>3 v\<^sub>4" by simp
+    ultimately show ?case by simp
+  qed simp_all
+
+lemma [simp]: "f\<^sub>l \<cdot> v \<Down> v' \<Longrightarrow> f\<^sub>l \<bar> f\<^sub>r \<cdot> InlV v \<Down> InlV v'"
+  proof
+    show "f\<^sub>l \<bar> f\<^sub>r \<cdot> InlV v \<leadsto> (\<iota>\<^sub>l \<cdot> f\<^sub>l) \<cdot> v" by simp
+    show "f\<^sub>l \<cdot> v \<Down> v' \<Longrightarrow> (\<iota>\<^sub>l \<cdot> f\<^sub>l) \<cdot> v \<Down> InlV v'" by auto
+  qed
+
+lemma [simp]: "f\<^sub>r \<cdot> v \<Down> v' \<Longrightarrow> f\<^sub>l \<bar> f\<^sub>r \<cdot> InrV v \<Down> InrV v'"
+  proof
+    show "f\<^sub>l \<bar> f\<^sub>r \<cdot> InrV v \<leadsto> (\<iota>\<^sub>r \<cdot> f\<^sub>r) \<cdot> v" by simp
+    show "f\<^sub>r \<cdot> v \<Down> v' \<Longrightarrow> (\<iota>\<^sub>r \<cdot> f\<^sub>r) \<cdot> v \<Down> InrV v'" by auto
+  qed
+
+(* since we are a turing-complete language, total progress is not provable *)
+
+theorem total_preservation: "e \<cdot> v \<Down> v' \<Longrightarrow> e \<turnstile> t\<^sub>1 \<rightarrow> t\<^sub>2 \<Longrightarrow> v \<turnstile> t\<^sub>1 \<Longrightarrow> v' \<turnstile> t\<^sub>2"
+  proof (induction e v v' arbitrary: t\<^sub>1 rule: total_eval.induct)
+  case (tev_step e v e' v' v'')
+    moreover then obtain t\<^sub>3 where "(e' \<turnstile> t\<^sub>3 \<rightarrow> t\<^sub>2) \<and> (v' \<turnstile> t\<^sub>3)" by (metis preservation)
+    ultimately show ?case by fastforce
+  qed auto
+
 end
